Add new level based comparison proof

Connect/ConProofComp.v
@@ -17,19 +17,36 @@ Local Opaque Z.add Z.mul Z.div Z.sub Z.land Z.lor Z.lxor Z.shiftl Z.shiftr Z.quo
 Require Import LayerSem.Libs.Zutils.BitOps.
 Require Import LayerSem.Libs.Zutils.hardcode_rewrite.
 
-(* Draft two *)
-(* removed dependency on level for walk and refrel, making them the same as walk_npt *)
-(* Uses Haddr_bound for boundary condition: see in set_refine *)
-(* Uses one of the rely clause for boundary condition:
-   see in set_refine
-   is_addr from both set and walk
-   rely from line 49 in S2PTTreeOps/Spec.v (level 2 empty for level 3 address)
-*)
+(* custom comparison vresion *)
 
-Definition addr_dec :=
-  forall addr addr',
-    is_addr addr -> is_addr addr' ->
-    {addr / 4096 = addr' / 4096} + {addr / 4096 / 512 <> addr' / 4096 / 512}.
+(* Pair Index Type *)
+Definition alpair := prod Z Z.
+
+(* Custom eq *)
+Definition eq_rel (x y : alpair) : Prop :=
+  let '(x1, x2) := x in
+  let '(y1, y2) := y in
+  if Z.eqb x2 y2 && Z.eqb x2 2 then
+    x1 / 4096 / 512  = y1 / 4096 / 512
+  else if Z.eqb x2 2 || Z.eqb y2 2 then
+    False
+  else
+    x1 / 4096 = y1 / 4096.
+Notation "x '$=' y" := (eq_rel x y) (at level 70).
+Notation "x '$<>' y" := (~ eq_rel x y) (at level 70).
+
+(* decidable for eq_rel *)
+Lemma al_eqdec : forall x y : alpair, {x $= y} + {x $<> y}.
+Proof.
+  intros [x1 x2] [y1 y2].
+  unfold eq_rel; simpl.
+  destruct ((x2 =? y2) && (x2 =? 2));
+  [|destruct ((x2 =? 2) || (y2 =? 2))];
+  match goal with
+  | [|- {?x = ?y} + {?x <> ?y}] => destruct (Z.eq_dec x y); auto
+  | [|- {False} + {~ False}] => right; auto
+  end.
+Qed.
 
 Definition pte_mask (pte: Z) : Z :=
   pte |' (1 << 55) |' (1 << 56).
@@ -79,7 +96,6 @@ Record refrel
   {
     id_same:
       forall addr,
-        is_addr addr ->
         let npt := hst.(shared).(e_s2pts) @ vmid in
         let r1 := walk vmid addr mem in
         let r2 :=
@@ -99,84 +115,70 @@ Record refrel
         end
   }.
 
-(* / 4096 / 512 <> -> / 4096 <> -> <> *)
-(* = -> / 4096 = -> / 4096 / 512 = *)
-(* satisfiability: easy <-> hard *)
-
 Theorem set_refine :
   forall {X : Type} vmid addr level pte pte' mem mem' mem'' hst hst'
       (walk : Z -> Z -> X -> option (Z * X))
       (set : Z -> Z -> Z -> Z -> X -> option X)
       (rel: Z -> Z -> Prop)
-    (* Boundary condition *)
-    (Haddr_bound: addr_dec)
     (* array propery *)
-    (Haneq:
-      forall addr' ,
-        (* is_addr addr' -> *)
-        addr' / 4096 / 512 <> addr / 4096 / 512 ->
-        (* addr' / 4096 / 512 <> addr / 4096 / 512 -> *)
-        fst_option (walk vmid addr' mem') = 
-        fst_option (walk vmid addr' mem))
-    (Haeq:
-      forall addr',
-        (* is_addr addr' -> *)
-        addr' / 4096 / 512 = addr / 4096 / 512 ->
-        (* addr' / 4096 / 512 = addr / 4096 / 512 -> *)
-        walk vmid addr' mem' = Some (pte', mem'') /\ rel pte' pte),
+    (Haneq: forall addr' level',
+        (addr', level') $<> (addr, level)->
+        walk vmid addr' mem' = 
+        walk vmid addr' mem)
+    (Haeq: forall addr' level', 
+      (addr', level') $= (addr, level)->
+      walk vmid addr' mem' = Some (pte', mem'') /\ rel pte' pte),
     (* goal *)
     refrel vmid hst walk mem rel ->
     set_npt_spec vmid addr level pte hst = Some hst' ->
     set vmid addr level pte mem = Some mem' ->
     refrel vmid hst' walk mem' rel.
 Proof.
-  intros X vmid addr level pte pte' mem mem' mem'' gst gst' walk set rel Haddr_bound Haneq Haeq Hrel Hspec Hspec2.
+  intros X vmid addr level pte pte' mem mem' mem'' gst gst' walk set rel
+  Haneq Haeq Hrel Hspec Hspec2.
   inv Hrel. constructor. intros.
   rename addr0 into addr'.
-  specialize (id_same0 addr' H) as id_same'.
+  (* specialize (id_same0 addr' level') as id_same'. *)
   unfold set_npt_spec in *.
   unfold walk_npt_spec in *.
   repeat autounfold with sem in *.
   repeat simpl_hyp Hspec;
   repeat simpl_hyp Hspec2.
   repeat extract_prop.
-  clear Prop0 Prop1 Prop3.
+  clear Prop0 Prop2 Prop1 Prop3.
   subst npt r1 r2.
   inv Hspec. simpl.
   rewrite ZMap.gsspec. rewrite zeq_true.
   simpl_func C3; repeat extract_prop. simpl.
   - simpl_func C1; repeat extract_prop.
-    clear Prop0 Prop1 Prop3. simpl.
-    destruct (Haddr_bound _ _ H Prop2) as [eq|neq].
+    clear Prop0 Prop1 Prop2. simpl.
+    destruct (al_eqdec (addr', level) (addr, level)) as [eq|neq].
     (* addr = addr' *)
-    + assert (addr' / 4096 / 512 = addr / 4096 / 512) as eq' by congruence.
-      specialize (Haeq _ eq') as [Haeq rel_low]. rewrite Haeq in *.
-      rewrite Z.eqb_eq in C. rewrite ZMap.gsspec. rewrite eq. rewrite zeq_true.
+    + specialize (Haeq _ _ eq) as [Haeq rel_low]. simpl in eq.
+      rewrite Z.eqb_refl in eq. rewrite C in eq. simpl in eq.
+      rewrite eq. rewrite ZMap.gsspec. rewrite zeq_true. rewrite Haeq.
       unfold refrel_pte. simpl. exists pte. unfold rel_pte.
       split; [assumption|solve_pte_mask].
     (* addr <> addr' *) 
-    + rewrite ZMap.gsspec. rewrite zeq_false; [|assumption].
-      specialize (Haneq _ neq). unfold fst_option in Haneq.
-      destruct (walk vmid addr' mem) as [ [v1 _]|];
-      destruct (walk vmid addr' mem') as [ [v2 _]|];
-      inversion Haneq; subst; apply id_same'.
+    + specialize (Haneq _ _ neq) as Haneq. simpl in neq.
+      rewrite Z.eqb_refl in neq. rewrite C in neq. simpl in neq.
+      rewrite ZMap.gsspec. rewrite zeq_false; [|assumption].
+      rewrite Haneq. apply id_same0.
   - simpl_func C0; repeat extract_prop. simpl.
     clear Prop1.
-    destruct (Haddr_bound _ _ H Prop2) as [eq|neq].
+    destruct (al_eqdec (addr', level) (addr, level)) as [eq|neq].
     (* addr = addr' *)
-    + assert (addr' / 4096 / 512 = addr / 4096 / 512) as eq' by congruence.
-      specialize (Haeq _ eq') as [Haeq rel_low]. rewrite Haeq.
-      subst. simpl in Prop0. rewrite eq in *. rewrite Prop0 in *.
-      rewrite ZMap.gsspec. rewrite zeq_true.
+    + specialize (Haeq _ _ eq) as [Haeq rel_low]. simpl in eq.
+      rewrite Z.eqb_refl in eq. rewrite C in eq. simpl in eq.
+      simpl in Prop0. rewrite eq in *. rewrite Prop0.
+      rewrite ZMap.gsspec. rewrite zeq_true. rewrite Haeq.
       unfold refrel_pte. simpl. exists pte. unfold rel_pte.
       split; [assumption|solve_pte_mask].
     (* addr <> addr' *)
-    + assert (addr' / 4096 <> addr / 4096) by congruence.
+    + specialize (Haneq _ _ neq) as Haneq. simpl in neq.
+      rewrite Z.eqb_refl in neq. rewrite C in neq. simpl in neq.
       rewrite ZMap.gsspec. rewrite zeq_false; [|assumption].
-      specialize (Haneq _ neq). unfold fst_option in Haneq.
-      destruct (walk vmid addr' mem) as [ [v1 _]|];
-      destruct (walk vmid addr' mem') as [ [v2 _]|];
-      inversion Haneq; subst; apply id_same'.
+      rewrite Haneq. apply id_same0.
 Qed.
 
 Theorem walk_refine:
@@ -184,27 +186,26 @@ Theorem walk_refine:
     (walk : Z -> Z -> X -> option (Z * X))
     (rel: Z -> Z -> Prop)
     (* array theory *)
-    (Hpure: forall addr',
-      (* is_addr addr' -> *)
-      fst_option (walk vmid addr' mem) = 
-      fst_option (walk vmid addr' mem')),
+    (Haeq: forall addr',
+        fst_option (walk vmid addr' mem) = 
+        fst_option (walk vmid addr' mem')),
     (* goal *)
     refrel vmid hst walk mem rel ->
     walk_npt_spec vmid addr hst = Some (v1, hst') ->
     walk vmid addr mem = Some (v2, mem') ->
-    refrel vmid hst' walk mem' rel /\ refrel_pte rel rel_pte v2 v1.
+    refrel vmid hst' walk mem' rel.
 Proof.
-  intros X vmid addr mem mem' hst hst' v1 v2 walk rel Hpure Hrel Hspec Hspec2.
+  intros X vmid addr mem mem' hst hst' v1 v2 walk rel Haeq Hrel Hspec Hspec2.
   unfold walk_npt_spec in *.
   repeat autounfold with sem in *.
   repeat simpl_hyp Hspec;
   repeat extract_prop.
-  clear Prop0 Prop1 Prop3. inv Hspec.
-  split.
+  clear Prop0 Prop1 Prop2 Prop3.
+  inv Hspec.
   (* refine rel *)
   inv Hrel. constructor. intros.
   rename id_same0 into id_same', addr0 into addr'.
-  specialize (id_same' addr' H).
+  specialize (id_same' addr').
   subst npt r1 r2. simpl in id_same'.
   remember (
     match (e_lv2pt (e_s2pts (shared hst')) @ vmid) @ (addr' / 4096 / 512) with
@@ -216,18 +217,12 @@ Proof.
           end
       end
   ) as r2.
-  specialize (Hpure addr').
+  specialize (Haeq addr').
   destruct (walk vmid addr' mem) as [p1|] eqn:Hg1;
   destruct (walk vmid addr' mem') as [p2|] eqn:Hg2;
-  simpl in Hpure;
   try (destruct p1);
   try (destruct p2);
+  simpl in Haeq;
   destruct r2;
   try congruence.
-  (* refine val *)
-  unfold s2pt_walk. inv Hrel. specialize (id_same0 _ Prop2) as id_same'; clear id_same0.
-  simpl in *. rewrite Hspec2 in id_same'.
-  destruct ((e_lv2pt (e_s2pts (shared hst')) @ vmid) @ (addr / 4096 / 512)); [assumption|].
-  destruct ((e_lv3pt (e_s2pts (shared hst')) @ vmid) @ (addr / 4096)); [assumption|].
-  inv id_same'.
 Qed.
